common/NatMapFacts.v
@@ -1,0 +1,26 @@
+(** * Facts about NatMap *)
+
+Require Import NatMap.
+
+(** Looks for two MapsTo proofs where the same key maps to two
+    different values that are structurally different (i.e, built from
+    two different constructors). *)
+
+Ltac mapsto_discriminate_simpl :=
+  lazymatch goal with
+  | [ H: MapsTo ?k ?v ?m, H': MapsTo ?k ?v' ?m |- _ ] =>
+    generalize (MapsTo_fun H H'); intros Heq;
+    tryif (assert_fails (discriminate Heq))
+    then fail "Term" v "=" v' "is not discriminable"
+    else discriminate Heq
+  | _ => fail "MapsTo proofs not found"
+  end.
+
+Ltac mapsto_discriminate_or :=
+  lazymatch goal with
+  | [ H: MapsTo ?k ?v ?m \/ MapsTo ?k ?v' ?m |- _ ] =>
+    inversion H; mapsto_discriminate_simpl
+  | _ => fail "Found no term matching MapsTo ?k ?v ?m \/ MapsTo ?k ?v' ?m"
+  end.
+
+Ltac mapsto_discriminate := mapsto_discriminate_simpl || mapsto_discriminate_or.
