hvhdl/Elaboration.v
@@ -1,0 +1,11 @@
+(** * Elaboration libraries *)
+
+Require Export DefaultValue.
+Require Export ConstraintElaboration.
+Require Export StaticExpressions.
+Require Export ExpressionEvaluation.
+Require Export TypeElaboration.
+Require Export GenericElaboration.
+Require Export PortElaboration.
+Require Export ArchitectureElaboration.
+Require Export DesignElaboration.
