soundness/InitialStates.v
@@ -1,18 +1,60 @@
 (** * Similar Initial States *)
 
+Require Import common.Coqlib.
 Require Import common.NatMap.
 
+Require Import sitpn.dp.Sitpn.
+Require Import sitpn.dp.SitpnTypes.
+Require Import sitpn.dp.SitpnSemanticsDefs.
 Require Import sitpn.dp.SitpnSemantics.
+Require Import sitpn.dp.SitpnFacts.
 
+Require Import hvhdl.HVhdlTypes.
 Require Import hvhdl.SemanticalDomains.
 Require Import hvhdl.DesignElaboration.
 Require Import hvhdl.AbstractSyntax.
 Require Import hvhdl.HilecopDesignStore.
 Require Import hvhdl.Initialization.
+Require Import hvhdl.Environment.
 
+Require Import sitpn2hvhdl.Sitpn2HVhdlTypes.
 Require Import sitpn2hvhdl.GenerateHVhdl.
 
 Require Import soundness.SoundnessDefs.
+
+(** ** Initial States Equal Marking Lemma *)
+
+Lemma init_states_eq_marking :
+  forall sitpn decpr id__ent id__arch mm d γ Δ σ__e σ0,
+    
+    (* [sitpn] translates into [(d, γ)]. *)
+    sitpn_to_hvhdl sitpn decpr id__ent id__arch mm = (inl (d, γ)) ->
+    
+    (* [Δ, σ__e] are the results of the elaboration of [d]. *)
+    edesign hdstore (empty value) d Δ σ__e ->
+
+    (* initialization d's state. *)
+    init Δ σ__e (behavior d) σ0 ->
+
+    forall p id__p σ__p0,
+      (* [id__p] is the identifier of the place component associated with
+         place [p] by the [γ] binder. *)
+      InA Pkeq (p, id__p) (p2pcomp γ) ->
+
+      (* [σ__p] is the current state of component [id__p] is the global
+         design state [σ]. *)
+      MapsTo id__p σ__p0 (compstore σ0) ->
+
+      (* Marking of place [p] at state [s] equals value of signal
+         [s_marking] at state [σ__p]. *)
+      MapsTo Place.s_marking (Vnat (M (s0 sitpn) p)) (sigstore σ__p0).
+Proof.
+  intros.
+
+  assert (Hv_initm_smark :
+            exists v, MapsTo Place.initial_marking v (sigstore σ__p0)
+                      /\ MapsTo Place.s_marking v (sigstore σ__p0)).
+Admitted.
 
 (** ** Similar Initial States Lemma *)
 
@@ -31,7 +73,8 @@ Lemma sim_init_states :
     (* init states are similar *)
     γ ⊢ (s0 sitpn) ∼ σ0.
 Proof.
-  
+  intros; unfold SimState. split.
+  eapply init_states_eq_marking; eauto.
 Admitted.
 
 Hint Resolve sim_init_states : core.
