test/hvhdl/Adder.v
@@ -1,0 +1,138 @@
+(** * H-VHDL Simple Adder Design *)
+
+Require Import common.Coqlib.
+Require Import common.NatSet.
+Require Import common.NatMap.
+Require Import common.NatMapFacts.
+
+Require Import hvhdl.AbstractSyntax.
+Require Import hvhdl.HVhdlTypes.
+Require Import hvhdl.Environment.
+Require Import hvhdl.Elaboration.
+Require Import hvhdl.SemanticalDomains.
+Require Import hvhdl.Petri.
+
+Local Open Scope abss_scope.
+Local Open Scope natset_scope.
+
+(** ** Input ports *)
+
+(** Input port identifiers *)
+
+Definition a : ident := 2.
+Definition b : ident := S a.
+
+(** Input port declarations *)
+
+Definition ins : list pdecl := [pdecl_in a tind_boolean; pdecl_in b tind_boolean].
+
+(** ** Output ports *)
+
+(** Out port identifiers *)
+
+Definition o : ident := S b.
+Definition outs : list pdecl := [pdecl_out o tind_boolean].
+
+(** ** Declared signals *)
+
+(** Declared signal identifiers *)
+
+Definition s_add : ident := S o.
+Definition sigs : list sdecl := [sdecl_ s_add tind_boolean].
+
+(** ** Adder behavior *)
+
+(** Process "add" (combinational) *)
+
+Definition add_ps_id : ident := S s_add.
+Definition add_ps : cs := cs_ps add_ps_id {[ a, b ]} [] (s_add @<== (#a @|| #b)).
+
+(** Process "publish" (synchronous) *)
+
+Definition publish_ps_id : ident := S add_ps_id.
+Definition publish_ps : cs := cs_ps publish_ps_id {[ clk, rst ]} [] (Falling (o @<== #s_add)).
+
+(** ** Adder design *)
+Definition adder_id__e : ident := S publish_ps_id.
+Definition adder_id__a : ident := S adder_id__e.
+Definition adder : design := design_ adder_id__e adder_id__a [] (ins ++ outs) sigs
+                                     (add_ps // publish_ps).
+Set Printing Coercions.
+
+Lemma vexpr_deterministic :
+  forall e Δ σ Λ mode v v',
+    vexpr Δ σ Λ mode e v ->
+    vexpr Δ σ Λ mode e v' -> v = v'.
+Proof.
+  induction e.
+  
+  (* CASE e is a nat constant *)
+  - do 2 inversion 1; auto.
+
+  (* CASE e is a bool constant *)
+  - do 2 inversion 1; auto.
+
+  (* CASE e is a name *)
+  - inversion 1.    
+    + inversion 1; eauto with mapsto.
+      -- admit. (* CASE id ∈ σ and id ∈ Λ, violates identifier unicity. *)
+      -- mapsto_discriminate. (* CASE id ∈ Gens(Δ) and id ∈ Sigs(Δ) ∪ Ins(Δ), impossible by def. *)
+    + inversion 1; eauto with mapsto.
+      -- admit. (* CASE id ∈ σ and id ∈ Λ, violates identifier unicity. *)
+      -- mapsto_discriminate. (* CASE id ∈ Gens(Δ) and id ∈ Outs(Δ), impossible by def. *)
+    + inversion 1; eauto with mapsto.
+      -- admit. (* CASE id ∈ σ and id ∈ Λ, violates identifier unicity. *)
+      -- admit. (* CASE id ∈ σ and id ∈ Λ, violates identifier unicity. *)
+      -- admit.
+      -- admit. (* CASE id ∈ σ and id ∈ Λ, violates identifier unicity. *)
+    + inversion 1; (eauto with mapsto || mapsto_discriminate || idtac).
+      -- admit. (* CASE id ∈ σ and id ∈ Λ, violates identifier unicity. *)
+      -- admit. (* CASE id ∈ σ and id ∈ Λ, violates identifier unicity. *)
+    + inversion 1.
+Admitted.
+
+Lemma econstr_eq_bounds :
+  forall Δ e e' n m n' m',
+    econstr Δ e e' n m -> econstr Δ e e' n' m' -> n = n' /\ m = m'.
+Proof.
+  intros Δ e e' n m n' m' Heconstr Heconstr'.
+  inversion Heconstr; inversion Heconstr'.
+
+    
+Lemma etype_eq_type : forall Δ τ t t', etype Δ τ t -> etype Δ τ t' -> t = t'.
+  intros Δ τ t t' Ht Ht'.
+  inversion Ht; inversion Ht';
+  (reflexivity || match goal with
+                 | [ Heq: _ = ?a, Heq': _ = ?a |- _ ] =>
+                   rewrite <- Heq in Heq';
+                   (discriminate
+                    || injection Heq'; intros Heqe Heqe'; rewrite Heqe, Heqe' in *)
+                 | _ => auto
+                  end).
+
+Lemma eport_defaultv :
+  forall Δ σ id τ Δ' σ' t v,
+    (eport Δ σ (pdecl_out id τ) Δ' σ' \/ eport Δ σ (pdecl_in id τ) Δ' σ') ->
+    etype Δ τ t ->
+    defaultv t v ->
+    MapsTo id v (sigstore σ').
+Proof.
+  intros Δ σ id τ Δ' σ' t v Hv_eport Hetype Hdv.
+  inversion_clear Hv_eport; inversion_clear H.
+Admitted.
+
+
+  
+Lemma adder_o_defaultv :
+  forall Δ__adder σ__e,
+    edesign (empty design) (empty value) adder Δ__adder σ__e ->
+    MapsTo o (Vbool false) (sigstore σ__e).
+Proof.
+  intros *; intros Helab.
+  inversion_clear Helab.
+  unfold outs in H0.
+  do 3 (match goal with
+        | [ H: eports _ _ _ _ _ |- _ ] => inversion_clear H
+        end).
+Admitted.
+
